certify_lift_diff WIP

src/refinement/SimCertify.v
@@ -29,52 +29,52 @@ Inductive sim_time (ts:Time.t) (v1 v2:Time.t): Prop :=
 .
 Hint Constructors sim_time.
 
-Inductive sim_view (ts:Time.t) (ex:Taint.t) (v1 v2:View.t (A:=Taint.t)): Prop :=
+Inductive sim_view (ts:Time.t) (forbid:Taint.t) (v1 v2:View.t (A:=Taint.t)): Prop :=
 | sim_view_intro
     (TS: v2.(View.ts) <= ts ->
          v1 = v2 /\
-         v2.(View.annot) ∩₁ ex ⊆₁ bot)
+         v2.(View.annot) ∩₁ forbid ⊆₁ bot)
 .
 Hint Constructors sim_view.
 
-Inductive sim_val (ts:Time.t) (ex:Taint.t) (v1 v2:ValA.t (A:=View.t (A:=Taint.t))): Prop :=
+Inductive sim_val (ts:Time.t) (forbid:Taint.t) (v1 v2:ValA.t (A:=View.t (A:=Taint.t))): Prop :=
 | sim_val_intro
     (TS: v2.(ValA.annot).(View.ts) <= ts ->
          v1 = v2 /\
-         v2.(ValA.annot).(View.annot) ∩₁ ex ⊆₁ bot)
+         v2.(ValA.annot).(View.annot) ∩₁ forbid ⊆₁ bot)
 .
 Hint Constructors sim_val.
 
-Inductive sim_rmap (ts:Time.t) (ex:Taint.t) (rmap1 rmap2:RMap.t (A:=View.t (A:=Taint.t))): Prop :=
+Inductive sim_rmap (ts:Time.t) (forbid:Taint.t) (rmap1 rmap2:RMap.t (A:=View.t (A:=Taint.t))): Prop :=
 | sim_rmap_intro
     (RMAP: IdMap.Forall2
-             (fun _ => (sim_val ts ex))
+             (fun _ => (sim_val ts forbid))
              rmap1 rmap2)
 .
 Hint Constructors sim_rmap.
 
-Inductive sim_state (ts:Time.t) (ex:Taint.t) (st1 st2:State.t (A:=View.t (A:=Taint.t))): Prop :=
+Inductive sim_state (ts:Time.t) (forbid:Taint.t) (st1 st2:State.t (A:=View.t (A:=Taint.t))): Prop :=
 | sim_state_intro
     (STMTS: st1.(State.stmts) = st2.(State.stmts))
-    (RMAP: sim_rmap ts ex st1.(State.rmap) st2.(State.rmap))
+    (RMAP: sim_rmap ts forbid st1.(State.rmap) st2.(State.rmap))
 .
 Hint Constructors sim_state.
 
-Inductive sim_lc (ts:Time.t) (ex:Taint.t) (lc1 lc2:Local.t (A:=Taint.t)): Prop :=
+Inductive sim_lc (ts:Time.t) (forbid:Taint.t) (lc1 lc2:Local.t (A:=Taint.t)): Prop :=
 | sim_lc_intro
     (COH: forall loc, sim_time ts (lc1.(Local.coh) loc) (lc2.(Local.coh) loc))
-    (VRP: sim_view ts ex lc1.(Local.vrp) lc2.(Local.vrp))
-    (VWP: sim_view ts ex lc1.(Local.vwp) lc2.(Local.vwp))
-    (VRM: sim_view ts ex lc1.(Local.vrm) lc2.(Local.vrm))
-    (VWM: sim_view ts ex lc1.(Local.vwm) lc2.(Local.vwm))
-    (VCAP: sim_view ts ex lc1.(Local.vcap) lc2.(Local.vcap))
-    (VREL: sim_view ts ex lc1.(Local.vrel) lc2.(Local.vrel))
+    (VRP: sim_view ts forbid lc1.(Local.vrp) lc2.(Local.vrp))
+    (VWP: sim_view ts forbid lc1.(Local.vwp) lc2.(Local.vwp))
+    (VRM: sim_view ts forbid lc1.(Local.vrm) lc2.(Local.vrm))
+    (VWM: sim_view ts forbid lc1.(Local.vwm) lc2.(Local.vwm))
+    (VCAP: sim_view ts forbid lc1.(Local.vcap) lc2.(Local.vcap))
+    (VREL: sim_view ts forbid lc1.(Local.vrel) lc2.(Local.vrel))
     (FWDBANK: forall loc,
         opt_rel
           (fun fwd1 fwd2 =>
              fwd2.(FwdItem.ts) <= ts ->
              (fwd1.(FwdItem.ts) = fwd2.(FwdItem.ts) /\
-              sim_view ts ex fwd1.(FwdItem.view) fwd2.(FwdItem.view) /\
+              sim_view ts forbid fwd1.(FwdItem.view) fwd2.(FwdItem.view) /\
               fwd1.(FwdItem.ex) = fwd2.(FwdItem.ex)))
           (lc1.(Local.fwdbank) loc) (lc2.(Local.fwdbank) loc))
     (EXBANK: opt_rel
@@ -85,40 +85,249 @@ Inductive sim_lc (ts:Time.t) (ex:Taint.t) (lc1 lc2:Local.t (A:=Taint.t)): Prop :
 .
 Hint Constructors sim_lc.
 
-Inductive sim_mem (tid:Id.t) (ts:Time.t) (ex:Taint.t) (mem1 mem2:Memory.t): Prop :=
+Inductive sim_mem (tid:Id.t) (ts:Time.t) (forbid:Taint.t) (mem1 mem2:Memory.t): Prop :=
 | sim_mem_intro
     mem_prefix mem1' mem2' msg
     (LEN: ts = length mem_prefix)
     (MEM: mem1 = mem_prefix ++ mem1')
     (MEM: mem2 = mem_prefix ++ msg :: mem2')
+    (TID: List.Forall (fun msg => msg.(Msg.tid) = tid) mem1')
+    (TID: List.Forall (fun msg => msg.(Msg.tid) = tid) mem2')
     (MSG: msg.(Msg.tid) <> tid)
-    (EX: ex = (fun taint => exists id, taint = Taint.R id 0))
+    (FORBID: forbid = (fun taint => exists id, taint = Taint.R id 0))
 .
 Hint Constructors sim_mem.
 
-Inductive sim_eu (tid:Id.t) (ts:Time.t) (ex:Taint.t) (eu1 eu2:ExecUnit.t (A:=Taint.t)): Prop :=
+Inductive sim_eu (tid:Id.t) (ts:Time.t) (forbid:Taint.t) (eu1 eu2:ExecUnit.t (A:=Taint.t)): Prop :=
 | sim_eu_intro
-    (STATE: sim_state ts ex eu1.(ExecUnit.state) eu2.(ExecUnit.state))
-    (LOCAL: sim_lc ts ex eu1.(ExecUnit.local) eu2.(ExecUnit.local))
-    (MEM: sim_mem tid ts ex eu1.(ExecUnit.mem) eu2.(ExecUnit.mem))
+    (STATE: sim_state ts forbid eu1.(ExecUnit.state) eu2.(ExecUnit.state))
+    (LOCAL: sim_lc ts forbid eu1.(ExecUnit.local) eu2.(ExecUnit.local))
+    (MEM: sim_mem tid ts forbid eu1.(ExecUnit.mem) eu2.(ExecUnit.mem))
 .
 Hint Constructors sim_eu.
 
-Inductive sim_aeu (tid:Id.t) (ts:Time.t) (ex:Taint.t) (aeu1 aeu2:AExecUnit.t): Prop :=
+Inductive sim_aeu (tid:Id.t) (ts:Time.t) (forbid:Taint.t) (aeu1 aeu2:AExecUnit.t): Prop :=
 | sim_aeu_intro
-    (EU: sim_eu tid ts ex aeu1.(AExecUnit.eu) aeu2.(AExecUnit.eu))
+    (EU: sim_eu tid ts forbid aeu1.(AExecUnit.eu) aeu2.(AExecUnit.eu))
     (AUX: aeu1.(AExecUnit.aux) = aeu2.(AExecUnit.aux))
-    (AUX_EX: aeu2.(AExecUnit.aux).(AExecUnit.taint) ∩₁ ex ⊆₁ bot)
+    (AUX_FORBID: aeu2.(AExecUnit.aux).(AExecUnit.taint) ∩₁ forbid ⊆₁ bot)
 .
 Hint Constructors sim_aeu.
 
+Inductive sim_event ts forbid: forall (e1 e2:Event.t (A:=View.t (A:=Taint.t))), Prop :=
+| sim_event_internal
+    ctrl1 ctrl2
+    (CTRL: sim_view ts forbid ctrl1 ctrl2):
+    sim_event ts forbid (Event.internal ctrl1) (Event.internal ctrl2)
+| sim_event_read
+    ex ord vloc1 vloc2 res1 res2
+    (VLOC: sim_val ts forbid vloc1 vloc2)
+    (RES: sim_val ts forbid res1 res2):
+    sim_event ts forbid (Event.read ex ord vloc1 res1) (Event.read ex ord vloc2 res2)
+| sim_event_write
+    ex ord vloc1 vloc2 vval1 vval2 res1 res2
+    (VLOC: sim_val ts forbid vloc1 vloc2)
+    (VVAL: sim_val ts forbid vval1 vval2)
+    (RES: sim_val ts forbid res1 res2):
+    sim_event ts forbid (Event.write ex ord vloc1 vval1 res1) (Event.write ex ord vloc2 vval2 res2)
+| sim_event_barrier
+    b:
+    sim_event ts forbid (Event.barrier b) (Event.barrier b)
+.
+
+Lemma sim_time_join
+      ts l1 l2 r1 r2
+      (VIEW1: sim_time ts l1 r1)
+      (VIEW2: sim_time ts l2 r2):
+  sim_time ts (join l1 l2) (join r1 r2).
+Proof.
+  inv VIEW1. inv VIEW2.
+  econs. intro X. unfold join, Time.join in X. apply Time.max_lub_iff in X. des.
+  eauto.
+Qed.
+
+Lemma sim_val_const
+      ts forbid c:
+  sim_val ts forbid (ValA.mk _ c bot) (ValA.mk _ c bot).
+Proof.
+  econs. s. i. splits; ss. ii. inv H0. ss.
+Qed.
+
+Lemma sim_view_bot
+      ts forbid:
+  sim_view ts forbid bot bot.
+Proof.
+  econs. i. splits; ss. ii. inv H0. ss.
+Qed.
+
+Lemma sim_view_const
+      ts forbid c:
+  sim_view ts forbid (View.mk c bot) (View.mk c bot).
+Proof.
+  econs. i. splits; ss. ii. inv H0. ss.
+Qed.
+
+Lemma sim_view_join
+      ts forbid l1 l2 r1 r2
+      (VIEW1: sim_view ts forbid l1 r1)
+      (VIEW2: sim_view ts forbid l2 r2):
+  sim_view ts forbid (join l1 l2) (join r1 r2).
+Proof.
+  destruct l1 as [lt1 lv1].
+  destruct l2 as [lt2 lv2].
+  destruct r1 as [rt1 rv1].
+  destruct r2 as [rt2 rv2].
+  inv VIEW1. inv VIEW2. ss.
+  econs. s. intro X. unfold join, Time.join in X. apply Time.max_lub_iff in X. des.
+  specialize (TS X). specialize (TS0 X0). des. inv TS. inv TS0.
+  splits; ss. ii. inv H. inv H0.
+  - apply TS2. ss.
+  - apply TS1. ss.
+Qed.
+
+Lemma sim_val_view ts forbid v1 v2
+      (VAL: sim_val ts forbid v1 v2):
+  sim_view ts forbid v1.(ValA.annot) v2.(ValA.annot).
+Proof.
+  inv VAL. econs. i. specialize (TS H). des. subst. ss.
+Qed.
+
+Lemma sim_rmap_expr
+      ts forbid rmap1 rmap2 e
+      (RMAP: sim_rmap ts forbid rmap1 rmap2):
+  sim_val ts forbid (sem_expr rmap1 e) (sem_expr rmap2 e).
+Proof.
+  induction e; s.
+  - apply sim_val_const.
+  - unfold RMap.find. inv RMAP. specialize (RMAP0 reg). inv RMAP0; ss.
+    apply sim_val_const.
+  - econs. s. i. inv IHe. specialize (TS H). des. splits; ss. congr.
+  - econs. s. i. unfold join, Time.join in H. apply Time.max_lub_iff in H. des.
+    inv IHe1. inv IHe2.
+    specialize (TS H). specialize (TS0 H0). des. splits; ss.
+    + congr.
+    + ii. inv H1. inv H2.
+      * apply TS2. ss.
+      * apply TS1. ss.
+Qed.
+
+Lemma sim_rmap_add
+      ts forbid rmap1 rmap2 v1 v2 r
+      (RMAP: sim_rmap ts forbid rmap1 rmap2)
+      (VAL: sim_val ts forbid v1 v2):
+  sim_rmap ts forbid (RMap.add r v1 rmap1) (RMap.add r v2 rmap2).
+Proof.
+  inv RMAP. econs. ii. unfold RMap.add. rewrite ? IdMap.add_spec.
+  condtac; ss. inversion e. subst. econs. ss.
+Qed.
+
+Lemma sim_lc_step
+      ts forbid tid
+      e2 mem1 mem2
+      (lc1 lc2 lc2':Local.t (A:=Taint.t))
+      (STEP:  Local.step e2 tid mem2 lc2 lc2')
+      (MEM: sim_mem tid ts forbid mem1 mem2)
+      (LC: sim_lc ts forbid lc1 lc2)
+      (EVENT: sim_event ts forbid e2 e2):
+  exists e1 lc1',
+    <<STEP: Local.step e1 tid mem1 lc1 lc1'>> /\
+    <<LC: sim_lc ts forbid lc1' lc2'>> /\
+    <<EVENT: sim_event ts forbid e1 e2>>.
+Proof.
+  inv LC. inv STEP.
+  - (* internal *)
+    inv LC. esplits.
+    + econs 1; ss.
+    + econs; ss. apply sim_view_join; ss.
+      admit. (* sim_view ctrl *)
+    + eauto.
+  - (* read *)
+    inv STEP0. destruct (le_dec ts0 ts).
+    + (* read from old msg. *)
+      esplits.
+      * econs 2; eauto. econs; eauto.
+        { etrans; [|exact COH0].
+          specialize (COH (ValA.val vloc)). inv COH. rewrite TS; ss.
+          etrans; eauto.
+        }
+        { admit. (* memory no_msgs *) }
+        { admit. (* memory read *) }
+      * econs; ss.
+        { i. rewrite ? fun_add_spec. condtac; ss. }
+        { apply sim_view_join; [by ss|].
+          instantiate (1 := ord). destruct (OrdR.ge ord OrdR.acquire_pc); eauto using sim_view_bot.
+          s. repeat apply sim_view_join.
+          - inv EVENT. inv VLOC. econs. i. specialize (TS H). des.
+            splits; ss.
+          - ss.
+          - destruct (OrdR.ge ord OrdR.acquire); ss. apply sim_view_bot.
+          - apply sim_view_bot.
+          - specialize (FWDBANK (ValA.val vloc)). inv FWDBANK.
+            + apply sim_view_const.
+            + admit. (* fwd *)
+        }
+        { admit. (* sim_view *) }
+        { admit. (* sim_view *) }
+        { admit. (* sim_view *) }
+        { admit. (* exbank *) }
+      * admit. (* event *)
+    + (* read from new msg. *)
+      admit.
+  - (* write *)
+    admit.
+  - (* write_failure *)
+    admit.
+  - (* isb *)
+    admit.
+  - (* dmbst *)
+    admit.
+  - (* dmbld *)
+    admit.
+  - (* dmbsy *)
+    admit.
+Admitted.
+
+Lemma sim_state_step
+      ts forbid e1 e2 (st1 st2 st2':State.t (A:=View.t (A:=Taint.t)))
+      (EVENT: sim_event ts forbid e1 e2)
+      (STEP: State.step e2 st2 st2')
+      (SIM: sim_state ts forbid st1 st2):
+  exists st1',
+    <<STEP: State.step e1 st1 st1'>> /\
+    <<SIM: sim_state ts forbid st1' st2'>>.
+Proof.
+  destruct st1 as [stmts1 rmap1].
+  destruct st2 as [stmts2 rmap2].
+  inv SIM. ss. subst. inv STEP; inv EVENT.
+  - inv CTRL. exploit TS; [by apply bot_spec|]. i. des. subst.
+    esplits; ss.
+    + econs 1; ss.
+    + econs; ss.
+  - inv CTRL. exploit TS; [by apply bot_spec|]. i. des. subst.
+    esplits; ss.
+    + econs 2; ss.
+    + econs; ss. apply sim_rmap_add; ss. apply sim_rmap_expr. ss.
+  - esplits; ss.
+    + econs 3; ss.
+      admit. (* sim_event dead end.. *)
+    + econs; ss. apply sim_rmap_add; ss.
+  - (* write *)
+    admit.
+  - (* barrier *)
+    admit.
+  - (* if *)
+    admit.
+  - (* dowhile *)
+    admit.
+Admitted.
+
 Lemma sim_aeu_step
-      tid ts ex aeu1 aeu2 aeu2'
-      (SIM: sim_aeu tid ts ex aeu1 aeu2)
+      tid ts forbid aeu1 aeu2 aeu2'
+      (SIM: sim_aeu tid ts forbid aeu1 aeu2)
       (STEP: AExecUnit.step tid aeu2 aeu2'):
   exists aeu1',
     <<STEP: AExecUnit.step tid aeu1 aeu1'>> /\
-    <<SIM: sim_aeu tid ts ex aeu1' aeu2'>>.
+    <<SIM: sim_aeu tid ts forbid aeu1' aeu2'>>.
 Proof.
   destruct aeu1 as [[[stmts1 rmap1] lc1 mem1] aux1].
   destruct aeu2 as [[[stmts2 rmap2] lc2 mem2] aux2].
@@ -136,8 +345,8 @@ Proof.
       * left. econs; ss.
         { instantiate (2 := Event.internal bot). s. econs 1. }
         econs; eauto. econs; eauto.
-      * econs; ss. econs; ss. econs; try by apply LOCAL0.
-        s. rewrite ? bot_join; try by apply View.order. apply LOCAL0.
+      * econs; ss. econs; ss. inv LOCAL0. econs; ss.
+        apply sim_view_join; ss. apply sim_view_bot.
     + (* assign *)
       inv LC.
       eexists (AExecUnit.mk (ExecUnit.mk _ _ _) _). esplits.
@@ -145,10 +354,8 @@ Proof.
         { instantiate (2 := Event.internal bot). s. econs 2. eauto. }
         econs; eauto. econs; eauto.
       * econs; ss. econs; ss.
-        { econs; ss. admit. (* sim_rmap add *) }
-        { econs; try by apply LOCAL0.
-          s. rewrite ? bot_join; try by apply View.order. apply LOCAL0.
-        }
+        { econs; ss. apply sim_rmap_add; ss. apply sim_rmap_expr. ss. }
+        { inv LOCAL0. econs; ss. eauto using sim_view_join, sim_view_bot. }
     + (* read *)
       admit.
     + (* fulfill *)
@@ -160,9 +367,9 @@ Proof.
         { instantiate (2 := Event.write _ _ _ _ _). s. econs 4; eauto. }
         econs 4; eauto. econs; eauto.
       * econs; ss; cycle 1.
-        { admit. (* join bot *) }
+        { ii. apply AUX_FORBID. inv H. econs; ss. inv H0; ss. }
         econs; ss.
-        { econs; ss. admit. (* sim_rmap add *) }
+        { econs; ss. apply sim_rmap_add; ss. apply sim_val_const. }
         { econs; try by apply LOCAL0. ss. }
     + (* isb *)
       admit.
@@ -179,9 +386,14 @@ Proof.
         { instantiate (2 := Event.internal _). s. econs 6; eauto. }
         econs; eauto. econs; eauto.
       * econs; ss. econs; ss.
-        { econs; ss. admit. (* sim_rmap add *) }
-        { econs; try by apply LOCAL0. s.
-          admit. (* sim_view join *)
+        { econs; ss.
+          exploit sim_rmap_expr; eauto. instantiate (1 := cond). i.
+          inv x0. exploit TS; cycle 1.
+          { i. des. rewrite x. ss. }
+          admit. (* not depend on big ts *)
+        }
+        { inv LOCAL0. econs; ss. apply sim_view_join; ss.
+          apply sim_val_view. apply sim_rmap_expr. ss.
         }
     + (* dowhile *)
       inv LC.
@@ -189,32 +401,25 @@ Proof.
       * left. econs; ss.
         { instantiate (2 := Event.internal bot). s. econs 7. ss. }
         econs; eauto. econs; eauto.
-      * econs; ss. econs; ss. econs; try by apply LOCAL0.
-        s. rewrite ? bot_join; try by apply View.order. apply LOCAL0.
+      * econs; ss. econs; ss. inv LOCAL0. econs; ss.
+        eauto using sim_view_join, sim_view_bot.
   - (* write_step *)
     admit.
 Admitted.
 
 Lemma sim_aeu_rtc_step
-      tid ts ex aeu1 aeu2 aeu2'
-      (SIM: sim_aeu tid ts ex aeu1 aeu2)
+      tid ts forbid aeu1 aeu2 aeu2'
+      (SIM: sim_aeu tid ts forbid aeu1 aeu2)
       (STEP: rtc (AExecUnit.step tid) aeu2 aeu2'):
   exists aeu1',
     <<STEP: rtc (AExecUnit.step tid) aeu1 aeu1'>> /\
-    <<SIM: sim_aeu tid ts ex aeu1' aeu2'>>.
+    <<SIM: sim_aeu tid ts forbid aeu1' aeu2'>>.
 Proof.
   revert aeu1 SIM. induction STEP.
   { i. esplits; eauto. }
   i. exploit sim_aeu_step; eauto. i. des.
   exploit IHSTEP; eauto. i. des.
   esplits; [|by eauto]. econs; eauto.
-Qed.
-
-Lemma init_sim_view
-      ts ex v:
-  sim_view ts ex (AExecUnit.init_view v) (AExecUnit.init_view v).
-Proof.
-  econs; ss. splits; ss. ii. inv H0. inv H1.
 Qed.
 
 Lemma certify_lift_diff
@@ -238,12 +443,12 @@ Proof.
       + econs; ss. econs. ii.
         unfold AExecUnit.init_rmap. rewrite IdMap.map_spec.
         destruct (IdMap.find id (State.rmap st1)); ss. econs. econs; ss.
-        splits; ss.
-        ii. inv H0. inv H1.
-      + unfold AExecUnit.init_lc. econs; ss; eauto using init_sim_view.
+        splits; ss. ii. inv H0. ss.
+      + unfold AExecUnit.init_lc, AExecUnit.init_view.
+        econs; ss; eauto using sim_view_const.
         * admit. (* TODO: bug on init vcap *)
         * i. destruct (Local.fwdbank lc1 loc); ss. econs; ss.
-          splits; ss. apply init_sim_view.
+          splits; ss. apply sim_view_const.
         * admit. (* TODO: bug on exbank rel *)
         * inv WF. inv LOCAL. ss.
     - ii. inv H. inv H0.
@@ -253,5 +458,5 @@ Proof.
     + inv SIM. inv EU. inv LOCAL. etrans; eauto.
     + inv SIM. congr.
   - ii. des. destruct lock as [loc from to guarantee]. ss. subst.
-    inv LOCK. ss. inv SIM. eapply AUX_EX. econs; cycle 1; eauto.
+    inv LOCK. ss. inv SIM. eapply AUX_FORBID. econs; cycle 1; eauto.
 Admitted.
